HigherLambdaModel/KInfinity.lean
@@ -1,6 +1,7 @@
 import HigherLambdaModel.KInfinity.NonTrivial
 import HigherLambdaModel.KInfinity.Construction
 import HigherLambdaModel.KInfinity.Properties
+import HigherLambdaModel.KInfinity.ContinuousSemantics
 import HigherLambdaModel.KInfinity.Examples
 
 /-!
